src/PlutusIR/Semantics/Static/Typing_sound_complete.v
@@ -9,15 +9,17 @@ From PlutusCert Require Import
     Equality
     Kinding.Checker.
 Require Import Coq.Lists.List.
+Import ListNotations.
+Require Import Coq.Bool.Bool.
 
 Fixpoint type_check (Δ : list (binderTyname * kind)) (Γ : list (binderName * ty)) (term : term) : (option ty) :=
     match term with
     | Var x => lookup x Γ >>= fun T => normaliser_Jacco T
     | LamAbs x T1 t => 
         normaliser_Jacco T1 >>= fun T1n =>
-        match type_check Δ ((x, T1n) :: Γ) t with
-        | Some T2 => Some (Ty_Fun T1n T2) (* TODO: no normalisation of T2? Is it always normal? In the has_type efinition it is called T2n, so maybe it is*)
-        | _ => None
+        match type_check Δ ((x, T1n) :: Γ) t, kind_check Δ T1 with
+        | Some T2, Some Kind_Base => Some (Ty_Fun T1n T2) (* TODO: no normalisation of T2? Is it always normal? In the has_type efinition it is called T2n, so maybe it is*)
+        | _, _ => None
         end
     | Apply t1 t2 => (* TODO: normalisation? *)
         match type_check Δ Γ t1, type_check Δ Γ t2 with
@@ -99,3 +101,114 @@ Fixpoint type_check (Δ : list (binderTyname * kind)) (Γ : list (binderName * t
             end 
     | _ => None
     end. (* TODO: normalisation? *)
+
+Theorem type_checking_sound : forall Δ Γ t ty,
+  type_check Δ Γ t = Some ty -> (Δ ,, Γ |-+ t : ty).
+Proof with (try apply kind_checking_sound; try apply normaliser_Jacco_sound; auto).
+  intros.
+  generalize dependent Γ.
+  generalize dependent Δ.
+  generalize dependent ty.
+  induction t; 
+    intros ty Δ Γ Htc; 
+    inversion Htc as [Htc']; 
+    unfold bind in Htc'; 
+    repeat destruct_match; 
+    inversion Htc'; 
+    subst.
+  - (* Let, later *) admit.
+  - (* Let later *) admit.
+  - apply T_Var with (T:= t)...
+  - apply T_TyAbs...
+  - apply T_LamAbs...
+  - eapply T_Apply.
+    + eapply IHt1; eauto.
+    + eapply IHt2; eauto.
+      apply Ty_eqb_eq in Heqb.
+      now subst.
+  - apply T_Constant.
+  - apply normaliser_Jacco_sound in Heqo.
+    now apply T_Builtin with (T := lookupBuiltinTy d).
+  - apply Kind_eqb_eq in Heqb0.
+    subst.
+    apply T_TyInst with (X := b) (K2 := k0) (T1n := t2) (T2n := t3)...
+  - apply Ty_eqb_eq in Heqb0.
+    rewrite andb_true_iff in Heqb.
+    destruct Heqb as [Heqb1 Heqb2].
+    apply Kind_eqb_eq in Heqb1.
+    apply Kind_eqb_eq in Heqb2.
+    inversion Htc'.
+    subst.
+    apply T_IWrap with (K := k1_5) (T0n := t5)...
+  - apply T_Unwrap with (Fn := t1_1) (Tn := t1_2) (K := k)...
+Admitted.
+
+(* Hmmm, why does this rewrite?? This helper lemma is of course temporary TODO *)
+Lemma test (T2n T1n : ty) Δ Γ t x :
+    type_check Δ ((x, T1n)::Γ) t = Some T2n -> match type_check Δ ((x, T1n)::Γ) t with 
+                    | Some T2 => Some (Ty_Fun T1n T2) 
+                    | None => None
+                end = Some (Ty_Fun T1n T2n). 
+Proof.
+    intros. now rewrite H.
+Qed.
+
+(* this doesnt work inline...*)
+Lemma oof2 X K Δ Γ t Tn :
+type_check ((X, K) :: Δ) Γ t = Some Tn ->
+ match type_check ((X, K) :: Δ) Γ t with
+| Some T => Some (Ty_Forall X K T)
+| None => None
+end = Some (Ty_Forall X K Tn).
+Proof.
+    intros.
+    rewrite H.
+    reflexivity.
+Qed.
+
+
+Theorem type_checking_complete : forall Δ Γ t ty,
+    (Δ ,, Γ |-+ t : ty) -> type_check Δ Γ t = Some ty.
+Proof.
+  intros.
+  induction H; simpl; auto.
+  - rewrite H.
+    now apply normaliser_Jacco_complete. 
+  - apply normaliser_Jacco_complete in H0; rewrite H0; simpl.
+    apply kind_checking_complete in H; rewrite H.
+    (* rewrite IHhas_type. Why does this not work?? *)
+    now apply test.
+  - rewrite IHhas_type1.
+    rewrite IHhas_type2.
+    now rewrite -> Ty_eqb_refl.
+  - (* easy with a lemma like test *)
+    now apply oof2.        
+  - rewrite IHhas_type.
+    apply kind_checking_complete in H0; rewrite H0.
+    rewrite -> Kind_eqb_refl.
+    apply normaliser_Jacco_complete in H1; rewrite H1; simpl.
+    now apply normaliser_Jacco_complete in H2; rewrite H2; simpl.
+  - apply kind_checking_complete in H; rewrite H.
+    apply kind_checking_complete in H1; rewrite H1.
+    rewrite IHhas_type.
+    rewrite Kind_eqb_refl; simpl.
+    apply normaliser_Jacco_complete in H0; rewrite H0; simpl.
+    apply normaliser_Jacco_complete in H2; rewrite H2; simpl.
+    apply normaliser_Jacco_complete in H3; rewrite H3; simpl.
+    now rewrite Ty_eqb_refl.
+  - rewrite IHhas_type.
+    apply kind_checking_complete in H0; rewrite H0.
+    now apply normaliser_Jacco_complete in H1; rewrite H1; simpl.
+  - subst.
+    now apply normaliser_Jacco_complete in H0; rewrite H0; simpl.
+  - (* error case, not implemented yet *) admit.
+  - (* let case: later *) admit.
+  - (* let rec case: later *) admit.
+Admitted.
+    
+
+
+
+      
+      
+      
